experiment/Experiment.Steel.Repr.ST.fst
@@ -5,7 +5,6 @@ module M    = Experiment.Steel.Repr.M
 module L    = FStar.List.Pure
 module Uv   = FStar.Universe
 module Dl   = Learn.DList
-module Lf   = Learn.ListFun
 module Perm = Learn.Permutation
 
 open Experiment.Steel.Repr.M
@@ -13,70 +12,33 @@ open Steel.Effect.Common
 
 
 type pre_t = Dl.ty_list
-type post_t (a : Type) = Lf.list_fun a Type
-unfold
-let  post_ts (#a : Type) (post : post_t a) : a -> Dl.ty_list = post.lf_list
-unfold
-let  post_t_of_ts (a : Type) : Dl.ty_list -> post_t a = Lf.const a
-unfold
-let  append_post_t (#a : Type) : post_t a -> post_t a -> post_t a = Lf.append #a #Type
+type post_t (a : Type) = a -> Dl.ty_list
 
 type req_t (pre : pre_t) = Dl.dlist pre -> prop
-type ens_t (pre : pre_t) (a : Type) (post : post_t a) = Dl.dlist pre -> (x : a) -> Dl.dlist (post_ts post x) -> prop
+type ens_t (pre : pre_t) (a : Type) (post : post_t a) = Dl.dlist pre -> (x : a) -> Dl.dlist (post x) -> prop
 
+let const_post (#a : Type) (ts : Dl.ty_list) : post_t a = fun _ -> ts
+let frame_post (#a : Type) (pt : post_t a) (fr : Dl.ty_list) : post_t a = fun (x : a) -> L.(pt x @ fr)
 
 noeq
 type prog_tree : (a : Type u#a) -> (pre : pre_t u#b) -> (post : post_t u#a u#b a) -> Type u#(1 + max a b) =
   | Tequiv : (pre : Dl.ty_list) -> (post : Dl.ty_list) ->
              (p : Perm.pequiv pre post) ->
-             prog_tree U.unit' pre (post_t_of_ts U.unit' post)
+             prog_tree U.unit' pre (const_post post)
   | Tspec  : (a : Type u#a) -> (pre : pre_t) -> (post : post_t a) -> (frame : Dl.ty_list) ->
              (req : req_t pre) -> (ens : ens_t pre a post) ->
-             prog_tree a L.(pre@frame) (append_post_t post (post_t_of_ts a frame))
+             prog_tree a L.(pre @ frame) (frame_post post frame)
   | Tret   : (a : Type u#a) -> (x : a) -> (post : post_t a) ->
-             prog_tree a (post_ts post x) post
+             prog_tree a (post x) post
   | Tbind  : (a : Type u#a) -> (b : Type u#a) ->
              (pre : pre_t) -> (itm : post_t a) -> (post : post_t b) ->
-             (f : prog_tree a pre itm) -> (g : ((x : a) -> prog_tree b (post_ts itm x) post)) ->
+             (f : prog_tree a pre itm) -> (g : ((x : a) -> prog_tree b (itm x) post)) ->
              prog_tree b pre post
   | TbindP : (a : Type u#a) -> (b : Type u#a) ->
              (pre : pre_t) -> (post : post_t b) ->
              (wp : pure_wp a) -> (x : unit -> PURE a wp) -> (g : a -> prog_tree b pre post) ->
              prog_tree b pre post
 
-noeq
-type shape_tree : (pre_n : nat) -> (post_n : nat) -> Type =
-  | Sequiv : (n : nat) -> (p : Perm.perm_f n) ->
-             shape_tree n n
-  | Sspec  : (pre_n : nat) -> (post_n : nat) -> (frame_n : nat) ->
-             shape_tree (pre_n + frame_n) (post_n + frame_n)
-  | Sret   : (n : nat) ->
-             shape_tree n n
-  | Sbind  : (pre_n : nat) -> (itm_n : nat) -> (post_n : nat) ->
-             (f : shape_tree pre_n itm_n) -> (g : shape_tree itm_n post_n) ->
-             shape_tree pre_n post_n
-  | SbindP : (pre_n : nat) -> (post_n : nat) ->
-             (g : shape_tree pre_n post_n) ->
-             shape_tree pre_n post_n
-
-let rec prog_has_shape (#a : Type u#a) (#pre : pre_t u#b) (#post : post_t u#a u#b a)
-                       (t : prog_tree a pre post) (s : shape_tree (L.length pre) (post.lf_len))
-  : Tot prop (decreases t)
-  = match t returns prop with
-  | Tequiv pre post p           -> s == Sequiv _ p
-  | Tspec  _ pre post frame _ _ -> s == Sspec  (L.length pre) (post.lf_len) (L.length frame)
-  | Tret   _ _ post             -> s == Sret   _
-  | Tbind  a _ pre itm post f g -> exists (s_f : shape_tree (L.length pre) itm.lf_len)
-                                    (s_g : shape_tree itm.lf_len     post.lf_len) .
-                                  s == Sbind _ _ _ s_f s_g /\
-                                  prog_has_shape f s_f /\
-                                  (forall (x : a) . prog_has_shape (g x) s_g)
-  | TbindP a _ pre post _ _ g   -> exists (s_g : shape_tree (L.length pre) post.lf_len) .
-                                  s == SbindP _ _ s_g /\
-                                  (forall (x : a) . prog_has_shape (g x) s_g)
-
-type prog_shape (#a : Type) (#pre : pre_t) (#post : post_t a) (t : prog_tree a pre post)
-  = s : shape_tree (L.length pre) (post.lf_len) {prog_has_shape t s}
 
 (* TODO ? r can requires t == t0*) 
 unfold
@@ -88,25 +50,25 @@ let match_prog_tree
       (c_Tequiv : (pre : Dl.ty_list) -> (post : Dl.ty_list) ->
                   (p : Perm.pequiv pre post) ->
                   Pure (r _ _ _ (Tequiv pre post p))
-                       (requires a0 == U.unit' /\ pre0 == pre /\ post0 == (post_t_of_ts U.unit' post) /\
+                       (requires a0 == U.unit' /\ pre0 == pre /\ post0 == const_post post /\
                                  t0 == Tequiv pre post p)
                        (ensures fun _ -> True))
       (c_Tspec  : (a : Type) -> (pre : pre_t) -> (post : post_t a) -> (frame : Dl.ty_list) ->
                   (req : req_t pre) -> (ens : ens_t pre a post) ->
                   Pure (r _ _ _ (Tspec a pre post frame req ens))
-                       (requires a0 == a /\ pre0 == L.(pre@frame) /\
-                                 post0 == append_post_t post (post_t_of_ts a frame) /\
+                       (requires a0 == a /\ pre0 == L.(pre @ frame) /\
+                                 post0 == frame_post post frame /\
                                  t0 == Tspec a pre post frame req ens)
                        (ensures fun _ -> True))
       (c_Tret   : (a : Type) -> (x : a) -> (post : post_t a) ->
                   Pure (r _ _ _ (Tret a x post))
-                       (requires a0 == a /\ pre0 == (post_ts post x) /\ post0 == post /\
+                       (requires a0 == a /\ pre0 == post x /\ post0 == post /\
                                  t0 == Tret a x post)
                        (ensures fun _ -> True))
       (c_Tbind  : (a : Type) -> (b : Type) ->
                   (pre : pre_t) -> (itm : post_t a) -> (post : post_t b) ->
                   (f : prog_tree a pre itm {f << t0}) ->
-                  (g : ((x : a) -> prog_tree b (post_ts itm x) post) {forall (x : a) . {:pattern (g x)} g x << t0}) ->
+                  (g : ((x : a) -> prog_tree b (itm x) post) {forall (x : a) . {:pattern (g x)} g x << t0}) ->
                   Pure (r _ _ _ (Tbind a b pre itm post f g))
                        (requires a0 == b /\ pre0 == pre /\ post0 == post /\
                                  t0 == Tbind a b pre itm post f g)
@@ -129,7 +91,7 @@ let match_prog_tree
 
 
 let bind (#a : Type) (#b : Type) (#pre : pre_t) (#itm : post_t a) (#post : post_t b)
-         (f : prog_tree a pre itm) (g : (x:a) -> prog_tree b (post_ts itm x) post)
+         (f : prog_tree a pre itm) (g : (x:a) -> prog_tree b (itm x) post)
   : prog_tree b pre post
   = Tbind a b pre itm post f g
 
@@ -145,7 +107,7 @@ let rec tree_req (#a : Type) (#pre : pre_t) (#post : post_t a) (t : prog_tree a 
              (fun sl0 -> True)
   | Tbind a _  _ itm _  f g ->
              (fun sl0 -> tree_req f sl0 /\
-               (forall (x : a) (sl1 : Dl.dlist (post_ts itm x)) . tree_ens f sl0 x sl1 ==> tree_req (g x) sl1))
+               (forall (x : a) (sl1 : Dl.dlist (itm x)) . tree_ens f sl0 x sl1 ==> tree_req (g x) sl1))
   | TbindP a _  _ _  wp _ g ->
              (fun sl0 -> wp (fun (x : a) -> tree_req (g x) sl0) /\ True)
 
@@ -157,16 +119,105 @@ and tree_ens (#a : Type) (#pre : pre_t) (#post : post_t a) (t : prog_tree a pre 
                sl1 == Dl.apply_pequiv p sl0)
   | Tspec a  pre post frame  req ens ->
              (fun sl0 x sl1 ->
-               let sl0', frame0 = Dl.splitAt_ty pre              frame sl0 in
-               let sl1', frame1 = Dl.splitAt_ty (post_ts post x) frame sl1 in
+               let sl0', frame0 = Dl.splitAt_ty pre      frame sl0 in
+               let sl1', frame1 = Dl.splitAt_ty (post x) frame sl1 in
                frame1 == frame0 /\ ens sl0' x sl1')
   | Tret _ x post ->
              (fun sl0 x' sl1 -> x' == x /\ sl1 == sl0)
   | Tbind a _  _ itm _  f g ->
              (fun sl0 y sl2 -> tree_req f sl0 /\
-               (exists (x : a) (sl1 : Dl.dlist (post_ts itm x)) . tree_ens f sl0 x sl1 /\ tree_ens (g x) sl1 y sl2))
+               (exists (x : a) (sl1 : Dl.dlist (itm x)) . tree_ens f sl0 x sl1 /\ tree_ens (g x) sl1 y sl2))
   | TbindP a _  _ _  wp _ g ->
              (fun sl0 y sl1 -> as_requires wp /\ (exists (x : a) . as_ensures wp x /\ tree_ens (g x) sl0 y sl1))
+
+
+(***** Shape *)
+
+noeq
+type shape_tree : (pre_n : nat) -> (post_n : nat) -> Type =
+  | Sequiv : (n : nat) -> (p : Perm.perm_f n) ->
+             shape_tree n n
+  | Sspec  : (pre_n : nat) -> (post_n : nat) -> (frame_n : nat) ->
+             shape_tree (pre_n + frame_n) (post_n + frame_n)
+  | Sret   : (n : nat) ->
+             shape_tree n n
+  | Sbind  : (pre_n : nat) -> (itm_n : nat) -> (post_n : nat) ->
+             (f : shape_tree pre_n itm_n) -> (g : shape_tree itm_n post_n) ->
+             shape_tree pre_n post_n
+  | SbindP : (pre_n : nat) -> (post_n : nat) ->
+             (g : shape_tree pre_n post_n) ->
+             shape_tree pre_n post_n
+
+let post_has_len (#a : Type) (post : post_t a) (len : nat) : prop = forall (x : a) . L.length (post x) = len
+
+let rec prog_has_shape (#a : Type u#a) (#pre : pre_t u#b) (#post : post_t u#a u#b a)
+                       (t : prog_tree a pre post)
+                       (#post_n : nat) (s : shape_tree (L.length pre) post_n)
+  : Pure prop (requires True)
+              (ensures fun p -> p ==> post_has_len post post_n)
+              (decreases t)
+  =
+    post_has_len post post_n /\
+    (match t returns prop with
+    | Tequiv pre post p           -> post_n = L.length pre /\ s == Sequiv _ p
+    | Tspec  _ pre post frame _ _ -> exists (post'_n : nat) .
+                                    post_n = post'_n + L.length frame /\
+                                    s == Sspec  (L.length pre) post'_n (L.length frame) /\
+                                    (forall (x : a) . L.length (post x) == post'_n)
+    | Tret   _ _ post             -> post_n = L.length pre /\
+                                    s == Sret   _
+    | Tbind  a b pre itm post f g -> exists (itm_n : nat)
+                                      (s_f : shape_tree (L.length pre) itm_n)
+                                      (s_g : shape_tree itm_n          post_n) .
+                                    s == Sbind _ _ _ s_f s_g /\
+                                    prog_has_shape f s_f /\
+                                    (forall (x : a) . prog_has_shape (g x) s_g)
+  | TbindP a _ pre post _ _ g   -> exists (s_g : shape_tree (L.length pre) post_n) .
+                                   s == SbindP _ _ s_g /\
+                                   (forall (x : a) . prog_has_shape (g x) s_g)
+  )
+
+let rec prog_has_shape' (#a : Type u#a) (#pre : pre_t u#b) (#post : post_t u#a u#b a)
+                        (t : prog_tree a pre post)
+                        (#post_n : nat) (s : shape_tree (L.length pre) post_n)
+  : Pure prop (requires True) (ensures fun p -> p <==> prog_has_shape t s) (decreases t)
+  = match t returns prop with
+  | Tequiv pre post p           -> (match s with
+                                  | Sequiv _ p' -> p' == p
+                                  | _ -> False)
+  | Tspec  _ pre post frame _ _ -> (match s with
+                                  | Sspec  pre_n post_n frame_n ->
+                                      pre_n = L.length pre /\
+                                     (forall (x : a) . post_n = L.length (post x)) /\
+                                      frame_n = L.length frame
+                                  | _ -> False)
+  | Tret   _ _ post             -> (match s with
+                                  | Sret   _ -> (forall (x : a) . post_n = L.length (post x))
+                                  | _ -> False)
+  | Tbind  a b pre itm post f g -> (match s with
+                                  | Sbind _ itm_n _ s_f s_g ->
+                                      prog_has_shape' f s_f /\
+                                      (forall (x : a) . prog_has_shape' (g x) s_g) /\
+                                      (forall (y : b) . post_n = L.length (post y))
+                                  | _ -> False)
+  | TbindP a b pre post _ _ g   -> (match s with
+                                  | SbindP _ _ s_g ->
+                                      (forall (x : a) . prog_has_shape' (g x) s_g) /\
+                                      (forall (y : b) . post_n = L.length (post y))
+                                  | _ -> False)
+
+
+noeq
+type prog_shape (#a : Type) (#pre : pre_t) (#post : post_t a) (t : prog_tree a pre post) = {
+  post_len : (l : nat {post_has_len post l});
+  shp      : (s : shape_tree (L.length pre) post_len {prog_has_shape t s});
+}
+
+unfold
+let mk_prog_shape (#a : Type) (#pre : pre_t) (#post : post_t a) (t : prog_tree a pre post)
+                  (#post_len : nat) (shp : shape_tree (L.length pre) post_len {prog_has_shape t shp})
+  : prog_shape t =
+  { post_len; shp}
 
 
 (*** Repr.M --> Repr.ST *)
@@ -174,13 +225,12 @@ and tree_ens (#a : Type) (#pre : pre_t) (#post : post_t a) (t : prog_tree a pre 
 module T = FStar.Tactics
 open FStar.Calc
 
-unfold
 let post_ST_of_M (#a : Type) (post : M.post_t a) : post_t a
-  = Lf.map Mkvprop'?.t post
+  = fun (x : a) -> vprop_list_sels_t (post x)
 
 let rec repr_ST_of_M (#a : Type u#a) (t : M.prog_tree a)
-                     (#pre : M.pre_t) (#post : M.post_t a) (c : M.tree_cond t pre post)
-  : Tot (prog_tree a (vprop_list_sels_t pre) (post_ST_of_M post))
+                     (#pre0 : M.pre_t) (#post0 : M.post_t a) (c : M.tree_cond t pre0 post0)
+  : Tot (prog_tree a (vprop_list_sels_t pre0) (post_ST_of_M post0))
         (decreases t)
   = match c with
   | TCspec #a #pre #post #req #ens  pre' post' frame  p0 p1 ->
@@ -188,13 +238,13 @@ let rec repr_ST_of_M (#a : Type u#a) (t : M.prog_tree a)
              (**) L.map_append Mkvprop'?.t pre frame;
              x <-- Tspec a (vprop_list_sels_t pre) (post_ST_of_M post)
                           (vprop_list_sels_t frame) req ens;
-             (**) L.map_append Mkvprop'?.t (post_vp post x) frame;
-             Tequiv (vprop_list_sels_t L.(post_vp post x@frame))
-                    (vprop_list_sels_t (post_vp post' x))
+             (**) L.map_append Mkvprop'?.t (post x) frame;
+             Tequiv (vprop_list_sels_t L.(post x @ frame))
+                    (vprop_list_sels_t (post' x))
                     (vequiv_sl (p1 x));;
              Tret _ x (post_ST_of_M post')
   | TCret #a #x  pre post  p ->
-             Tequiv (vprop_list_sels_t pre) (vprop_list_sels_t (post_vp post x)) (vequiv_sl p);;
+             Tequiv (vprop_list_sels_t pre) (vprop_list_sels_t (post x)) (vequiv_sl p);;
              Tret _ x (post_ST_of_M post)
   | TCbind #a #b #f #g  pre itm post  cf cg ->
              x <-- repr_ST_of_M f cf;
@@ -203,9 +253,26 @@ let rec repr_ST_of_M (#a : Type u#a) (t : M.prog_tree a)
              TbindP a b _ _ wp x (fun x -> repr_ST_of_M (g x) (cg x))
 
 
+let rec shape_ST_of_M (#pre_n : nat) (#post_n : nat) (s : M.shape_tree pre_n post_n)
+  : Tot (shape_tree pre_n post_n) (decreases s)
+  = match s with
+  | M.Sspec pre_n post_n frame_n p0 p1 ->
+        Sbind _ _ _ (Sequiv (pre_n  + frame_n) p0) (
+        Sbind _ _ _ (Sspec  pre_n post_n frame_n) (
+        Sbind _ _ _ (Sequiv (post_n + frame_n) p1)
+                    (Sret   (post_n + frame_n))))
+  | M.Sret n p ->
+        Sbind _ _ _ (Sequiv n p) (Sret n)
+  | M.Sbind _ _ _ f g -> Sbind  _ _ _ (shape_ST_of_M f) (shape_ST_of_M g)
+  | M.SbindP _ _ g    -> SbindP _ _ (shape_ST_of_M g)
+                    
+
+
+(***** soundness of M --> ST *)
+
 let norm_tree_spec () : T.Tac unit
-  = T.norm [delta_only [`%repr_ST_of_M; `%bind; `%tree_req; `%tree_ens];
-            delta_attr [`%Lf.__list_fun__; `%U.__util_func__];
+  = T.norm [delta_only [`%repr_ST_of_M; `%post_ST_of_M; `%bind; `%tree_req; `%tree_ens; `%const_post];
+            delta_attr [`%U.__util_func__];
             delta_qualifier ["unfold"];
             zeta; iota; simplify]
 
@@ -213,32 +280,33 @@ let norm_tree_spec () : T.Tac unit
 let repr_ST_of_M__TCspec_ens
       #a #pre #post (req : M.req_t pre) (ens : M.ens_t pre a post)
       (pre' : M.pre_t) (post' : M.post_t a) (frame : vprop_list)
-      (p0 : vequiv pre' L.(pre @ frame)) (p1 : (x : a) -> vequiv (post_vp post x @ frame) (post_vp post' x))
-      (sl0' : sl_t pre') (res : a) (sl1' : sl_t (post_vp post' res))
+      (p0 : vequiv pre' L.(pre @ frame)) (p1 : (x : a) -> vequiv (post x @ frame) (post' x))
+      (sl0' : sl_t pre') (res : a) (sl1' : sl_t (post' res))
 
   : Lemma (
     (**) L.map_append Mkvprop'?.t pre frame;
-    (**) L.map_append Mkvprop'?.t (post_vp post res) frame;
+    (**) L.map_append Mkvprop'?.t (post res) frame;
 
     (tree_ens (repr_ST_of_M _ (TCspec #a #pre #post #req #ens  pre' post' frame  p0 p1)) sl0' res sl1'
     <==> (let sl0, frame0 = Dl.splitAt_ty (vprop_list_sels_t pre) (vprop_list_sels_t frame)
                              (Dl.apply_pequiv (vequiv_sl p0) sl0') in
-        let sl1, frame1 = Dl.splitAt_ty (vprop_list_sels_t (post_vp post res)) (vprop_list_sels_t frame)
+        let sl1, frame1 = Dl.splitAt_ty (vprop_list_sels_t (post res)) (vprop_list_sels_t frame)
                              (Dl.apply_pequiv (Perm.pequiv_sym (vequiv_sl (p1 res))) sl1') in
         req sl0 /\ frame1 == frame0 /\ ens sl0 res sl1)))
   =
     L.map_append Mkvprop'?.t pre frame;
-    L.map_append Mkvprop'?.t (post_vp post res) frame;
+    L.map_append Mkvprop'?.t (post res) frame;
     assert (
       tree_ens (repr_ST_of_M _ (TCspec #a #pre #post #req #ens  pre' post' frame  p0 p1)) sl0' res sl1'
-    <==> (exists (sl1f : Dl.dlist L.(vprop_list_sels_t (post_vp post res) @ vprop_list_sels_t frame)) .
+    <==> (exists (sl1f : Dl.dlist L.(vprop_list_sels_t (post res) @ vprop_list_sels_t frame)) .
           let sl0, frame0 = Dl.splitAt_ty (vprop_list_sels_t pre) (vprop_list_sels_t frame)
                                (Dl.apply_pequiv (vequiv_sl p0) sl0') in
-          let sl1, frame1 = Dl.splitAt_ty (vprop_list_sels_t (post_vp post res)) (vprop_list_sels_t frame) sl1f in
+          let sl1, frame1 = Dl.splitAt_ty (vprop_list_sels_t (post res)) (vprop_list_sels_t frame) sl1f in
           sl1' == Dl.apply_pequiv (vequiv_sl (p1 res)) sl1f /\
           req sl0 /\ frame1 == frame0 /\ ens sl0 res sl1))
       by T.(norm_tree_spec (); smt ());
-    introduce forall (sl1f : Dl.dlist L.(vprop_list_sels_t (post_vp post res) @ vprop_list_sels_t frame)) .
+
+    introduce forall (sl1f : Dl.dlist L.(vprop_list_sels_t (post res) @ vprop_list_sels_t frame)) .
         sl1' == Dl.apply_pequiv (vequiv_sl (p1 res)) sl1f <==>
         sl1f == Dl.apply_pequiv (Perm.pequiv_sym (vequiv_sl (p1 res))) sl1'
       with Dl.apply_pequiv_sym_eq_iff (vequiv_sl (p1 res)) sl1f sl1';
@@ -246,7 +314,7 @@ let repr_ST_of_M__TCspec_ens
     assert (tree_ens (repr_ST_of_M _ (TCspec #a #pre #post #req #ens  pre' post' frame  p0 p1)) sl0' res sl1'
     <==> (let sl0, frame0 = Dl.splitAt_ty (vprop_list_sels_t pre) (vprop_list_sels_t frame)
                              (Dl.apply_pequiv (vequiv_sl p0) sl0') in
-        let sl1, frame1 = Dl.splitAt_ty (vprop_list_sels_t (post_vp post res)) (vprop_list_sels_t frame)
+        let sl1, frame1 = Dl.splitAt_ty (vprop_list_sels_t (post res)) (vprop_list_sels_t frame)
                              (Dl.apply_pequiv (Perm.pequiv_sym (vequiv_sl (p1 res))) sl1') in
         req sl0 /\ frame1 == frame0 /\ ens sl0 res sl1))
 #pop-options
@@ -300,7 +368,7 @@ let rec repr_ST_of_M_req (#a : Type) (t : M.prog_tree a)
                bind_req (M.tree_req f cf) (M.tree_ens f cf) (fun x -> M.tree_req (g x) (cg x)) sl0;
              <==> {
                repr_ST_of_M_req f cf sl0;
-               introduce forall (x : a) (sl1 : sl_t (post_vp itm x)) .
+               introduce forall (x : a) (sl1 : sl_t (itm x)) .
                  tree_req (repr_ST_of_M f cf) sl0 ==>
                  (M.tree_ens f cf sl0 x sl1 <==> tree_ens (repr_ST_of_M f cf) sl0 x sl1) /\
                  (M.tree_req (g x) (cg x) sl1 <==> tree_req (repr_ST_of_M (g x) (cg x)) sl1)
@@ -308,7 +376,7 @@ let rec repr_ST_of_M_req (#a : Type) (t : M.prog_tree a)
                with _ . (repr_ST_of_M_ens f cf sl0 x sl1; repr_ST_of_M_req (g x) (cg x) sl1)
              }
                tree_req (repr_ST_of_M f cf) sl0 /\
-               (forall (x : a) (sl1 : Dl.dlist (vprop_list_sels_t (post_vp itm x))) .
+               (forall (x : a) (sl1 : Dl.dlist (vprop_list_sels_t (itm x))) .
                  tree_ens (repr_ST_of_M f cf) sl0 x sl1 ==> tree_req (repr_ST_of_M (g x) (cg x)) sl1);
              <==> {_ by T.(apply_lemma (`U.iff_refl); trefl ())}
                tree_req (repr_ST_of_M _ (TCbind #a #b #f #g  pre itm post  cf cg)) sl0;
@@ -340,25 +408,25 @@ let rec repr_ST_of_M_req (#a : Type) (t : M.prog_tree a)
 
 and repr_ST_of_M_ens (#a : Type) (t : M.prog_tree a)
                      (#pre : M.pre_t) (#post : M.post_t a) (c : M.tree_cond t pre post)
-                     (sl0 : sl_t pre) (res : a) (sl1 : sl_t (post_vp post res))
+                     (sl0 : sl_t pre) (res : a) (sl1 : sl_t (post res))
   : Lemma (requires M.tree_req t c sl0)
           (ensures M.tree_ens t c sl0 res sl1 <==> tree_ens (repr_ST_of_M t c) sl0 res sl1)
   = match c as c returns squash (M.tree_ens t c sl0 res sl1 <==> tree_ens (repr_ST_of_M t c) sl0 res sl1) with
     | TCspec #a #pre #post #req #ens  pre' post' frame  p0 p1 ->
              L.map_append Mkvprop'?.t pre frame;
-             L.map_append Mkvprop'?.t (post_vp post res) frame;
+             L.map_append Mkvprop'?.t (post res) frame;
 
              calc (<==>) {
                M.tree_ens _ (TCspec #a #pre #post #req #ens  pre' post' frame  p0 p1) sl0 res sl1;
              <==> {_ by T.(apply_lemma (`U.iff_refl); trefl ()) }
               (let fsl0, frame0 = extract_vars_f pre' pre frame p0 sl0 in
-               let fsl1, frame1 = extract_vars_f (post_vp post' res) (post_vp post res) frame
+               let fsl1, frame1 = extract_vars_f (post' res) (post res) frame
                                                  (Perm.pequiv_sym (p1 res)) sl1 in
                 frame1 == frame0 /\ ens fsl0 res fsl1);
              <==> { (* since req holds *) }
               (let fsl0, frame0 = Dl.splitAt_ty (vprop_list_sels_t pre) (vprop_list_sels_t frame)
                                                   (Dl.apply_pequiv (vequiv_sl p0) sl0) in
-               let fsl1, frame1 = Dl.splitAt_ty (vprop_list_sels_t (post_vp post res)) (vprop_list_sels_t frame)
+               let fsl1, frame1 = Dl.splitAt_ty (vprop_list_sels_t (post res)) (vprop_list_sels_t frame)
                                                   (Dl.apply_pequiv (Perm.pequiv_sym (vequiv_sl (p1 res))) sl1) in
                 req fsl0 /\ frame1 == frame0 /\ ens fsl0 res fsl1);
              <==> {repr_ST_of_M__TCspec_ens req ens pre' post' frame p0 p1 sl0 res sl1}
@@ -393,7 +461,7 @@ and repr_ST_of_M_ens (#a : Type) (t : M.prog_tree a)
                bind_ens (M.tree_req f cf) (M.tree_ens f cf) (fun x -> M.tree_ens (g x) (cg x)) sl0 res sl1;
              <==> {
                repr_ST_of_M_req f cf sl0;
-               introduce forall (x : a) (sl1' : sl_t (post_vp itm x)) .
+               introduce forall (x : a) (sl1' : sl_t (itm x)) .
                  tree_req (repr_ST_of_M f cf) sl0 ==>
                  (M.tree_ens f cf sl0 x sl1' <==> tree_ens (repr_ST_of_M f cf) sl0 x sl1') /\
                  (M.tree_ens f cf sl0 x sl1' ==> (
@@ -404,7 +472,7 @@ and repr_ST_of_M_ens (#a : Type) (t : M.prog_tree a)
                 with _ . repr_ST_of_M_ens (g x) (cg x) sl1' res sl1
              }
                tree_req (repr_ST_of_M f cf) sl0 /\
-               (exists (x : a) (sl1' : Dl.dlist (vprop_list_sels_t (post_vp itm x))) .
+               (exists (x : a) (sl1' : Dl.dlist (vprop_list_sels_t (itm x))) .
                  tree_ens (repr_ST_of_M f cf) sl0 x sl1' /\
                  tree_ens (repr_ST_of_M (g x) (cg x)) sl1' res sl1);
              <==> {_ by T.(apply_lemma (`U.iff_refl); trefl ())}
@@ -444,50 +512,35 @@ and repr_ST_of_M_ens (#a : Type) (t : M.prog_tree a)
 #pop-options
 
 
+let repr_ST_of_M_shape__norm : list norm_step =
+  [delta_only [`%prog_has_shape'; `%repr_ST_of_M; `%shape_ST_of_M; `%bind];
+   iota; zeta]
 
-(* --------------------------- *)
-
-open Steel.Reference
-
-let test_ST (r : ref nat) = repr_ST_of_M (test_M r).repr_tree (test_cond r)
-
-//let _ = fun r ->
-// assert (print_util (test_ST r))
-//    by T.(norm normal_spec_steps; qed ())
-
-let test_ST_shape =
-  Sbind 1 1 1 (Sbind 1 1 1 (Sequiv 1 (Perm.id_n 1))
-              (Sbind 1 1 1 (Sspec  1 1 0)
-              (Sbind 1 1 1 (Sequiv 1 (Perm.id_n 1))
-                           (Sret   1))))
-              (Sbind 1 1 1 (Sequiv 1 (Perm.id_n 1))
-                           (Sret   1))
-
-let rec prog_has_shape' (#a : Type u#a) (#pre : pre_t u#b) (#post : post_t u#a u#b a)
-                        (t : prog_tree a pre post) (s : shape_tree (L.length pre) (post.lf_len))
-  : Pure prop (requires True) (ensures fun p -> p <==> prog_has_shape t s) (decreases t)
-  = match t returns prop with
-  | Tequiv pre post p           -> (match s with
-                                  | Sequiv _ p' -> p' == p
-                                  | _ -> False)
-  | Tspec  _ pre post frame _ _ -> (match s with
-                                  | Sspec  pre_n post_n frame_n ->
-                                      pre_n == L.length pre /\ post_n == post.lf_len /\ frame_n == L.length frame
-                                  | _ -> False)
-  | Tret   _ _ post             -> (match s with
-                                  | Sret   _ -> True
-                                  | _ -> False)
-  | Tbind  a _ pre itm post f g -> (match s with
-                                  | Sbind _ itm_n _ s_f s_g ->
-                                      itm_n == itm.lf_len /\
-                                      prog_has_shape' f s_f /\
-                                      (forall (x : a) . prog_has_shape' (g x) s_g)
-                                  | _ -> False)
-  | TbindP a _ pre post _ _ g   -> (match s with
-                                  | SbindP _ _ s_g -> (forall (x : a) . prog_has_shape' (g x) s_g)
-                                  | _ -> False)
-
-
-let test_ST_has_shape (r : ref nat)
-  : squash (prog_has_shape' (test_ST r) test_ST_shape)
-  = _ by T.(norm normal_spec_steps; norm [simplify]; smt ())
+#push-options "--ifuel 1"
+let rec repr_ST_of_M_shape
+      (#a : Type) (t : M.prog_tree a)
+      (#pre : M.pre_t) (#post : M.post_t a) (c : M.tree_cond t pre post)
+      (#post_n : nat) (s : M.shape_tree (L.length pre) post_n)
+   : Lemma (requires M.tree_cond_has_shape c s)
+           (ensures  prog_has_shape (repr_ST_of_M t c) (shape_ST_of_M s))
+   = match c with
+   | TCspec #a #pre #post #req #ens pre1 post1 frame p0 p1 ->
+            let M.Sspec pre_n post_n frame_n p0' p1' = s in
+            assert (prog_has_shape' (repr_ST_of_M t (TCspec #a #pre #post #req #ens pre1 post1 frame p0 p1))
+                                    (shape_ST_of_M (M.Sspec pre_n post_n frame_n p0' p1')))
+                by T.(norm repr_ST_of_M_shape__norm; smt ())
+  | TCret #a #x pre post p ->
+            let M.Sret n p' = s in
+            assert (prog_has_shape' (repr_ST_of_M t (TCret #a #x pre post p))
+                                    (shape_ST_of_M (M.Sret n p')))
+                by T.(norm repr_ST_of_M_shape__norm; smt ())
+  | TCbind #a #b #f #g _ _ _ cf cg ->
+            let M.Sbind _ _ _ s_f s_g = s in
+            repr_ST_of_M_shape f cf s_f;
+            introduce forall (x : a) . prog_has_shape (repr_ST_of_M (g x) (cg x)) (shape_ST_of_M s_g)
+              with repr_ST_of_M_shape (g x) (cg x) s_g
+  | TCbindP #a #b #_ #_ #g _ _ cg ->
+            let M.SbindP _ _ s_g = s in
+            introduce forall (x : a) . prog_has_shape (repr_ST_of_M (g x) (cg x)) (shape_ST_of_M s_g)
+              with repr_ST_of_M_shape (g x) (cg x) s_g
+#pop-options
